GenericModuleLib/SharedDataDefs.v
@@ -1,0 +1,425 @@
+(* %%%%%%%%%%%%%%%%%%%%%%%%%%%%%%%%%%%%%%%%%%%%%%%%%%%%%%%%%%%%%%%%% *) 
+(* Module with shared definitions used by 
+   "interfaces" and "implementations".
+  
+   Last Update: Mon, 22 May 2017
+ %%%%%%%%%%%%%%%%%%%%%%%%%%%%%%%%%%%%%%%%%%%%%%%%%%%%%%%%%%%%%%%%%%% *) 
+
+Add LoadPath "../..".
+
+Require Import ConceptParams.AuxTactics.LibTactics.
+Require Import ConceptParams.AuxTactics.BasicTactics.
+
+Require Import ConceptParams.SetMapLib.List2Set.
+Require Import ConceptParams.SetMapLib.ListPair2FMap.
+
+Require Import Coq.Lists.List.
+Import ListNotations.
+Require Import Coq.Bool.Bool.
+
+Require Import Coq.Structures.Orders.
+Require Import Coq.Structures.Equalities.
+
+(* ***************************************************************** *)
+(** * Shared Data Definitions *)
+
+(** Data definition shared by various kinds of modules *)
+(* ***************************************************************** *)
+(* ***************************************************************** *)
+
+(* ################################################################# *)
+(** ** Data Module Types  *)
+(* ################################################################# *)
+
+(** Wrapper module for a single type *)
+Module Type Data.
+  (** Type of Data *)
+  Parameter t : Type.
+End Data.
+
+(** Module consisting of types of _Data_ and _Context_ *)
+Module Type DataC.
+  (** Type of Data *)
+  Parameter t : Type.
+  (** Type of Context (might be needed for checking WD of [t]) *)
+  Parameter ctx : Type.
+End DataC.
+
+(** Module consisting of types of 
+ ** _Data_, _global context_, and _Local Context_ *)
+Module Type DataLC.  
+  (** Type of Data *)
+  Parameter t : Type.
+  (** Type of Context (might be needed for checking WD of [t]) *)
+  Parameter ctx : Type.
+  (** Type of Local Context which might also be needed
+   ** for checking WD of [t] *)
+  Parameter ctxloc : Type.
+End DataLC.
+
+
+(* ################################################################# *)
+(** ** Module Types for Well-definedness of Modules *)
+(* ################################################################# *)
+
+(* ================================================================= *)
+(** ** Module Types for Well-definedness of Simple Modules *)
+
+(** In a _Simple Module_ all elements are checked independently 
+ ** of each other: only global context matters. *)
+(* ================================================================= *)
+
+Module Type DataCOkDef (Import D : DataC).
+  Parameter is_ok : ctx -> t -> Prop.
+End DataCOkDef.
+
+Module Type DataCOkInterp (Import D : DataC).
+  Parameter is_ok_b : ctx -> t -> bool.
+End DataCOkInterp.
+
+Module Type DataCOkProp (Import D : DataC) 
+       (Import DDef : DataCOkDef D) (Import DInt : DataCOkInterp D).
+
+  Axiom is_ok_b__sound : forall (c : ctx) (x : t),
+      is_ok_b c x = true -> is_ok c x.
+  Axiom is_ok_b__complete : forall (c : ctx) (x : t),
+      is_ok c x -> is_ok_b c x = true.
+End DataCOkProp.
+
+(* ================================================================= *)
+(** ** Module Types with Well-definedness of Single-Pass Modules *)
+
+(** In a _Single-Pass Module_ following elements can refer to
+ ** the previously defined ones by means of the local context. *)
+(* ================================================================= *)
+
+Module Type DataLCOkDef (Import D : DataLC). 
+  (* Element [t] must be ok with respect 
+     to global [ctx] and local [ctxloc] contexts. *) 
+  Parameter is_ok : ctx -> ctxloc -> t -> Prop.
+End DataLCOkDef.
+
+Module Type DataLCOkInterp (Import D : DataLC).
+  Parameter is_ok_b : ctx -> ctxloc -> t -> bool.
+End DataLCOkInterp.
+
+Module Type DataLCOkProp (Import D : DataLC) 
+       (Import DDef : DataLCOkDef D) (Import DInt : DataLCOkInterp D).
+
+  Axiom is_ok_b__sound : forall (c : ctx) (cl : ctxloc) (x : t),
+    is_ok_b c cl x = true -> is_ok c cl x.
+  
+  Axiom is_ok_b__complete : forall (c : ctx) (cl : ctxloc) (x : t),
+    is_ok c cl x -> is_ok_b c cl x = true.
+End DataLCOkProp.
+
+
+(* ################################################################# *)
+(** ** Shared Parameters of all building blocks *)
+(* ################################################################# *)
+
+Module Type IdentifiersBase.
+  (* Id Set *)
+  Declare Module IdDT  : UsualDecidableType.
+  Declare Module IdSET : MSetInterface.WSets
+           with Definition E.t := IdDT.t
+           with Definition E.eq := IdDT.eq.
+  Declare Module IdLS  : List2MSet IdDT IdSET.
+  
+  (* Id Map *)
+  Declare Module IdDT' : ListPair2FMap.UsualDecidableTypeOrig
+      with Definition t  := IdDT.t
+      with Definition eq := IdDT.eq.
+  Declare Module IdMAP : FMapInterface.WS 
+           with Definition E.t := IdDT.t
+           with Definition E.eq := IdDT.eq.
+  Declare Module IdLPM : ListPair2FMapW IdDT' IdMAP.
+
+  (* Id *)
+  Definition id := IdDT.t.
+(*Definition id_set := IdLS.id_set.
+  Definition id_map := IdLPM.id_map.*)
+End IdentifiersBase.
+
+
+(* ################################################################# *)
+(** ** Module Types for Modules *)
+(* ################################################################# *)
+
+Module Type ModuleBase.
+  Declare Module MId : IdentifiersBase.
+  Definition id := MId.id.
+  Definition id_set := MId.IdLS.id_set.
+  Definition id_map := MId.IdLPM.id_map.
+End ModuleBase.
+
+
+(* ################################################################# *)
+(** ** Generic Well-definedness of Modules *)
+(* ################################################################# *)
+
+Module Type GenericModule_Data.
+  (** Type of members *)
+  Parameter dt : Type.
+  (** Type of context *)
+  Parameter ctx : Type.
+End GenericModule_Data.
+
+
+Module Type GenericModule_DataDefs (Import MId : IdentifiersBase) 
+       (Import MD : GenericModule_Data).
+  Parameter members_ok : ctx -> list (id * dt) -> Prop.
+End GenericModule_DataDefs.
+
+Module Type GenericModule_DataInterp (Import MId : IdentifiersBase) 
+       (Import MD : GenericModule_Data).
+  Parameter members_ok_b : ctx -> list (id * dt) -> bool.
+End GenericModule_DataInterp.
+
+Module Type GenericModule_DataProps (Import MId : IdentifiersBase) 
+       (Import MD  : GenericModule_Data)
+       (Import MDD : GenericModule_DataDefs MId MD)
+       (Import MDI : GenericModule_DataInterp MId MD)
+.
+  Axiom members_ok_b__sound : forall (c : ctx) (decls : list (id * dt)),
+    members_ok_b c decls = true -> members_ok c decls.
+  
+  Axiom members_ok_b__complete : forall (c : ctx) (decls : list (id * dt)),
+    members_ok c decls -> members_ok_b c decls = true.
+End GenericModule_DataProps.
+
+
+Module GenericModule_Defs (Import MId : IdentifiersBase) 
+       (Import MD  : GenericModule_Data)
+       (Import MDD : GenericModule_DataDefs MId MD).
+
+  Definition module_ok (c : ctx) (decls : list (id * dt)) : Prop :=
+    let nms := map fst decls in
+    (** all names are distinct *)
+    List.NoDup nms
+    (** and all members are valid *)
+    /\ members_ok c decls. 
+
+End GenericModule_Defs.
+
+Module GenericModule_Interp (Import MId : IdentifiersBase) 
+       (Import MD : GenericModule_Data)
+       (Import MDI : GenericModule_DataInterp MId MD).
+
+  Definition module_ok_b (c : ctx) (decls : list (id * dt)) : bool :=
+    let nms := map fst decls in
+    andb
+      (** all names are distinct *)
+      (MId.IdLS.ids_are_unique nms)
+      (** and all types are valid *)
+      (members_ok_b c decls).
+
+End GenericModule_Interp.
+
+Module GenericModule_Props (Import MId : IdentifiersBase) 
+       (Import MD : GenericModule_Data)
+       (Import MDD : GenericModule_DataDefs MId MD)
+       (Import MDI : GenericModule_DataInterp MId MD)
+       (Import MDP : GenericModule_DataProps MId MD MDD MDI).
+
+  Module MDef := GenericModule_Defs   MId MD MDD.
+  Module MInt := GenericModule_Interp MId MD MDI.
+  Import MDef. Import MInt.
+
+  Theorem module_ok_b__sound : forall (c : ctx) (decls : list (id * dt)),
+      module_ok_b c decls = true ->
+      module_ok c decls.
+  Proof.
+    intros c ds. intros H.
+    unfold module_ok_b in H. 
+    unfold module_ok.
+    rewrite -> andb_true_iff in H. inversion H as [Hid Hds].
+    apply MId.IdLS.Props.ids_are_unique__sound in Hid.
+    apply members_ok_b__sound in Hds.
+    split; assumption.
+  Qed.
+
+  Theorem module_ok_b__complete : forall (c : ctx) (decls : list (id * dt)),
+      module_ok c decls ->
+      module_ok_b c decls = true.
+  Proof.
+    intros c ds. intros H.
+    unfold module_ok_b.
+    unfold module_ok in H.
+    inversion H as [Hdup Hmems].
+    rewrite -> andb_true_iff. split.
+    apply MId.IdLS.Props.ids_are_unique__complete in Hdup. assumption.
+    apply members_ok_b__complete. assumption.
+  Qed.  
+
+End GenericModule_Props.
+
+
+
+
+
+
+Module GenericModuleData (Import MId : IdentifiersBase).
+  
+  (** Type of members *)
+  Parameter dt : Type.
+  (** Type of context *)
+  Parameter ctx : Type.
+
+  Parameter members_ok   : ctx -> list (id * dt) -> Prop.
+
+  Definition module_ok (c : ctx) (decls : list (id * dt)) : Prop :=
+    let nms := map fst decls in
+    (** all names are distinct *)
+    List.NoDup nms
+    (** and all members are valid *)
+    /\ members_ok c decls. 
+
+  Parameter members_ok_b : ctx -> list (id * dt) -> bool.
+
+  Definition module_ok_b (c : ctx) (decls : list (id * dt)) : bool :=
+    let nms := map fst decls in
+    andb
+      (** all names are distinct *)
+      (MId.IdLS.ids_are_unique nms)
+      (** and all types are valid *)
+      (members_ok_b c decls).
+
+  Axiom members_ok_b__sound : forall (c : ctx) (decls : list (id * dt)),
+    members_ok_b c decls = true -> members_ok c decls.
+  
+  Axiom members_ok_b__complete : forall (c : ctx) (decls : list (id * dt)),
+    members_ok c decls -> members_ok_b c decls = true.
+
+  Theorem module_ok_b__sound : forall (c : ctx) (decls : list (id * dt)),
+      module_ok_b c decls = true ->
+      module_ok c decls.
+  Proof.
+    intros c ds. intros H.
+    unfold module_ok_b in H. 
+    unfold module_ok.
+    rewrite -> andb_true_iff in H. inversion H as [Hid Hds].
+    apply MId.IdLS.Props.ids_are_unique__sound in Hid.
+    apply members_ok_b__sound in Hds.
+    split; assumption.
+  Qed.
+
+  Theorem module_ok_b__complete : forall (c : ctx) (decls : list (id * dt)),
+      module_ok c decls ->
+      module_ok_b c decls = true.
+  Proof.
+    intros c ds. intros H.
+    unfold module_ok_b.
+    unfold module_ok in H.
+    inversion H as [Hdup Hmems].
+    rewrite -> andb_true_iff. split.
+    apply MId.IdLS.Props.ids_are_unique__complete in Hdup. assumption.
+    apply members_ok_b__complete. assumption.
+  Qed.  
+
+End GenericModuleData.
+
+
+
+
+
+(* ################################################################# *)
+(** ** Old *)
+(* ################################################################# *)
+
+Module Type DataOkDef (D : DataC) := DataCOkDef D.
+Module Type DataOkInterp (D : DataC) := DataCOkInterp D.
+Module Type DataOkProp (D : DataC) 
+       (DDef : DataCOkDef D) (DInt : DataCOkInterp D) :=
+  DataCOkProp D DDef DInt.
+
+
+Module Type IntrfsBase.
+  Include IdentifiersBase.
+
+  (* Types Data *)
+  Declare Module TyDT : DataC.
+  Definition ty := TyDT.t.
+
+  Definition intrfs_ast := list (id * ty).
+  Definition intrfs_map := IdLPM.id_map ty.
+
+  Parameter members_to_define : intrfs_map -> list id.
+End IntrfsBase.
+
+Module Type IntrfsLCBase.
+  Include IdentifiersBase.
+
+  (* Types Data *)
+  Declare Module TyDT : DataLC.
+  Definition ty := TyDT.t.
+
+  Definition intrfs_ast := list (id * ty).
+  Definition intrfs_map := IdLPM.id_map ty.
+End IntrfsLCBase.
+
+
+
+
+(* ################################################################# *)
+(** ** Module Types  *)
+(* ################################################################# *)
+
+(** Data which might depend on some local context. *)
+Module Type DepData.  
+  (** Contains types [t] and [ctx] *)
+  Include DataC. 
+
+  (** Type of local context which might be
+      required for checking a  *)
+  Parameter ctxloc : Type.
+End DepData.
+
+Module Type DepDataOkDef (Import D : DepData) 
+       (Import MI : IntrfsBase).
+  (* Element [id] = [t] must be ok with respect 
+     to global [ctx] and local [ctxloc] contexts, and it also should 
+     correspond to the interface represented by [intrfs_map] *) 
+  Parameter is_ok : ctx -> intrfs_map -> ctxloc -> 
+                    id -> t -> Prop.
+End DepDataOkDef.
+
+Module Type DepDataOkInterp (Import D : DepData)
+       (Import MI : IntrfsBase).
+  Parameter is_ok_b : ctx -> intrfs_map -> ctxloc -> 
+                      id -> t -> bool.
+End DepDataOkInterp.
+
+Module Type DepDataOkProp (Import D : DepData) 
+       (Import MI : IntrfsBase)
+       (Import DDef : DepDataOkDef D MI) (Import DInt : DepDataOkInterp D MI).
+
+  Axiom is_ok_b__sound : 
+    forall (c : ctx) (imap : MI.intrfs_map) (cl : ctxloc)
+           (nm : id) (x : t),
+      is_ok_b c imap cl nm x = true -> is_ok c imap cl nm x.
+
+  Axiom is_ok_b__complete : 
+    forall (c : ctx) (imap : MI.intrfs_map) (cl : ctxloc) 
+           (nm : id) (x : t),
+      is_ok c imap cl nm x -> is_ok_b c imap cl nm x = true.
+End DepDataOkProp.
+
+
+
+(* ################################################################# *)
+(** ** Shared Parameters of all building blocks *)
+(* ################################################################# *)
+
+
+Module Type ImplmnBase (Import MI : IntrfsBase).
+  (** Module of a corresponding interface (the data depends on) *)
+(*  Declare Module MI : IntrfsBase. *)
+
+  (* Terms Data *) 
+  Declare Module TmDT : DepData.
+  Definition tm := TmDT.t.
+
+  Definition implmn_ast := list (id * tm).
+  Definition implmn_map := IdLPM.id_map tm.
+End ImplmnBase.
