GenericModuleLib/SinglePassModule.v
@@ -1,0 +1,411 @@
+(* %%%%%%%%%%%%%%%%%%%%%%%%%%%%%%%%%%%%%%%%%%%%%%%%%%%%%%%%%%%%%%%%% *) 
+(* Module with Certified Checking 
+   of Single-Pass Module.
+  
+   Last Update: Tue, 23 May 2017
+ %%%%%%%%%%%%%%%%%%%%%%%%%%%%%%%%%%%%%%%%%%%%%%%%%%%%%%%%%%%%%%%%%%% *) 
+
+Add LoadPath "../..".
+
+Require Import ConceptParams.AuxTactics.LibTactics.
+Require Import ConceptParams.AuxTactics.BasicTactics.
+
+Require Import ConceptParams.SetMapLib.List2Set.
+Require Import ConceptParams.SetMapLib.ListPair2FMap.
+
+Require Import ConceptParams.GenericModuleLib.SharedDataDefs.
+
+Require Import Coq.Lists.List.
+Import ListNotations.
+Require Import Coq.Bool.Bool.
+
+Require Import Coq.Structures.Orders.
+Require Import Coq.Structures.Equalities.
+
+(* ***************************************************************** *)
+(** * Single-Pass Module *)
+
+(** Single-Pass Module is well-defined if
+    all names are different 
+    and all members are well-defined with following elements
+      refering to the previously defined ones via local context. *)
+(* ***************************************************************** *)
+(* ***************************************************************** *)
+
+(* ################################################################# *)
+(** ** Shared Parameters of all building blocks *)
+(* ################################################################# *)
+
+Module Type SinglePassModuleBase.
+  Include ModuleBase.
+
+  Declare Module MD : DataLC.
+  Definition dt := MD.t.
+  Definition ctx := MD.ctx.
+  Definition ctxloc := MD.ctxloc.
+
+  (** Initial local context *)
+  Parameter ctxl_init : ctxloc.
+  (** Update local context *)
+  Parameter upd_ctxloc : ctxloc -> ctx -> id -> dt -> ctxloc.
+End SinglePassModuleBase.
+
+Module SinglePassModule_Data (MMB : SinglePassModuleBase) 
+<: GenericModule_Data. 
+
+  Definition dt := MMB.dt.
+  Definition ctx := MMB.ctx.
+End SinglePassModule_Data.
+
+(* ################################################################# *)
+(** ** Propositional Part *)
+(* ################################################################# *)
+
+Module SinglePassModuleDefs (Import MMB : SinglePassModuleBase) 
+       (Import TOkD : DataLCOkDef MMB.MD).
+
+  Module HelperD.
+
+    (** Aux function checking one member (to be used in [fold_left]).
+     ** The [okAndCl] param is an accumulator. *)
+    Definition process_dep_member (c : ctx) 
+               (okAndCl : Prop * ctxloc) (decl : id * dt) 
+               : Prop * ctxloc := 
+      match okAndCl with (ok_prop, cl) =>
+      match decl with (nm, d) =>
+        let ok_prop' := 
+            (* check curr member in the local context *)
+            TOkD.is_ok c cl d  
+            (* and preserve previous members' part *)
+            /\ ok_prop in
+        (* update local context *)
+        let cl' := MMB.upd_ctxloc cl c nm d in
+        (ok_prop', cl')
+      end end.
+
+    (** Aux function checking that all members are ok 
+     ** in the given initial conditions.
+     ** The [initP] parameter can be any provable proposition.
+          This is more convenient for doing proofs than 
+          using [True] as initial proposition, for example. *)
+    Definition members_ok' (c : ctx) (cl : ctxloc) (initP : Prop)
+               (decls : list (id * dt)) : Prop * ctxloc :=
+      List.fold_left (process_dep_member c) decls (initP, cl).
+
+    (** Aux function checking that all members are ok. *)
+    Definition members_ok (c : ctx) (decls : list (id * dt)) : Prop :=
+      fst (members_ok' c ctxl_init True decls).
+
+    Module MData := SinglePassModule_Data MMB.
+    Module MDataM <: GenericModule_DataDefs MId MData. 
+      Definition members_ok := members_ok.
+    End MDataM.
+    Module M := GenericModule_Defs MId MData MDataM.
+ 
+  End HelperD.
+
+  (** Single-Pass Module given as the AST [decls]  
+   ** is well-defined in the context [c]. *)
+  Definition module_ok (c : ctx) (decls : list (id * dt)) : Prop :=
+    HelperD.M.module_ok c decls.
+  (*  let nms := map fst decls in
+    (** all names are distinct *)
+    List.NoDup nms
+    (** and all members are valid *)
+    /\ HelperD.members_ok c decls. *)
+    
+
+End SinglePassModuleDefs.
+
+(* ################################################################# *)
+(** ** Computable Part (static checker of the interpreter) *)
+(* ################################################################# *)
+
+Module SinglePassModuleInterp (Import MMB : SinglePassModuleBase) 
+       (Import TOkI : DataLCOkInterp MMB.MD).
+
+  Module HelperI.
+
+    (** Aux function checking one member (to be used in [fold_left]).
+     ** The [okAndCl] param is an accumulator. *)
+    Definition process_dep_member_b (c : ctx) 
+               (okAndCl : bool * ctxloc) (decl : id * dt) 
+               : bool * ctxloc := 
+      match okAndCl with 
+      | (true, cl) =>
+        match decl with (nm, d) =>
+          let ok := TOkI.is_ok_b c cl d in
+          let cl' := MMB.upd_ctxloc cl c nm d in
+          (ok, cl')
+        end 
+      | (false, cl) => (false, cl)
+      end.
+
+    (** Aux function checking that all members are ok 
+     ** in the given initial conditions. *)
+    Definition members_ok'_b (c : ctx) (cl : ctxloc) 
+               (decls : list (id * dt)) : bool * ctxloc :=
+      List.fold_left (process_dep_member_b c) decls (true, cl).
+
+    (** Aux function checking that all members are ok. *)
+    Definition members_ok_b (c : ctx) (decls : list (id * dt)) : bool :=
+      fst (members_ok'_b c ctxl_init decls).
+
+    Module MData := SinglePassModule_Data MMB.
+    Module MDataM <: GenericModule_DataInterp MId MData. 
+      Definition members_ok_b := members_ok_b.
+    End MDataM.
+    Module M := GenericModule_Interp MId MData MDataM.
+
+  End HelperI.
+
+  (** Checks that a module given as the AST [decls]  
+   ** is well-defined in the context [c]. *)
+  Definition module_ok_b (c : ctx) (decls : list (id * dt)) : bool :=
+    HelperI.M.module_ok_b c decls.
+  (*  let nms := map fst decls in
+    andb
+      (** all names are distinct *)
+      (MId.IdLS.ids_are_unique nms)
+      (** and all types are valid *)
+      (HelperI.members_ok_b c decls). *)
+
+End SinglePassModuleInterp.
+
+(* ################################################################# *)
+(** ** Proofs of Correctness *)
+(* ################################################################# *)
+
+Module SinglePassModuleProps 
+       (Import MMB : SinglePassModuleBase)
+       (Import TOkD : DataLCOkDef MMB.MD)
+       (Import TOkI : DataLCOkInterp MMB.MD)
+       (Import TOkP : DataLCOkProp MMB.MD TOkD TOkI)
+.
+  Module Import MMD := SinglePassModuleDefs   MMB TOkD.
+  Module Import MMI := SinglePassModuleInterp MMB TOkI.
+  Import MMD.HelperD. Import MMI.HelperI.
+
+(* ----------------------------------------------------------------- *)
+(** *** Helper Props  *)
+(* ----------------------------------------------------------------- *)
+
+  Module Helper.
+    Import MMD.HelperD.
+    
+    (** Soundness *)   
+
+    Lemma process_dep_member_b_preserves_false :
+      forall (c : ctx) (decls : list (id * dt)) (cl : ctxloc),
+        fold_left (process_dep_member_b c) decls (false, cl) = (false, cl).
+    Proof.
+      intros c ds.
+      induction ds as [| [nm d] ds' IHds'];
+        intros cl.
+      - (* ds = nil *)
+        simpl. reflexivity.
+      - (* ds = (nm, d) :: ds' *)
+        simpl. apply IHds'.
+    Qed.
+
+    Lemma members_ok'_b_cons_true :
+      forall (c : ctx) (decls : list (id * dt)) (cl : ctxloc)
+             (nm : id) (d : dt),
+        fst (members_ok'_b c cl ((nm, d) :: decls)) = true ->
+        fst (members_ok'_b c (upd_ctxloc cl c nm d) decls) = true.
+    Proof.
+      intros c ds.
+      unfold members_ok'_b. simpl.
+      intros cl nm d H.
+      assert (Hok : is_ok_b c cl d = true).
+      { destruct (is_ok_b c cl d) eqn:Heq.
+        reflexivity.
+        destruct ds as [| elem ds'].
+        + simpl in H. assumption.
+        + rewrite (process_dep_member_b_preserves_false c _ _) in H.
+          simpl in H. inversion H. }
+      rewrite Hok in H. assumption.
+    Qed.
+
+    Lemma members_ok'_b_true__head_ok :
+      forall (c : ctx) (decls : list (id * dt)) (cl : ctxloc)
+             (nm : id) (d : dt),
+        fst (members_ok'_b c cl ((nm, d) :: decls)) = true ->
+        is_ok_b c cl d = true.
+    Proof.
+      intros c ds cl nm d H.
+      unfold members_ok'_b in H. simpl in H.
+      destruct (is_ok_b c cl d) eqn:Heq.
+      reflexivity.
+      rewrite (process_dep_member_b_preserves_false c _ _) in H.
+      simpl in H. assumption.
+    Qed. 
+
+    Lemma members_ok'_b__sound :
+      forall (c : ctx) (decls : list (id * dt)) (cl : ctxloc) (initP : Prop),
+        initP ->
+        fst (members_ok'_b c cl decls) = true ->
+        fst (members_ok' c cl initP decls).
+    Proof.
+      intros c ds.
+      induction ds as [| [nm t] ds' IHds'];
+        intros cl P HP H.
+      - simpl. assumption.
+      - (* ds = (nm, t) :: ds' *)
+        assert (H' := H).
+        apply members_ok'_b_true__head_ok in H'.
+        assert (H'' := H').
+        apply TOkP.is_ok_b__sound in H''.
+        unfold members_ok'. simpl.
+        apply IHds'.
+        tauto.
+        unfold members_ok'_b in H. simpl in H.
+        unfold members_ok'_b. rewrite H' in H. 
+        assumption.
+    Qed.
+
+(* ----------------------------------------------------------------- *) 
+
+    (** Completeness *)
+
+    Lemma members_ok'__fst_prop :
+      forall (c : ctx) (decls : list (id * dt)) (cl : ctxloc) (initP : Prop)
+             (nm : id) (d : dt),
+      exists Ps : Prop,
+        (fst (members_ok' c cl initP ((nm, d) :: decls)) = Ps)
+        /\ (Ps -> (is_ok c cl d) /\ initP).
+    Proof.
+      intros c ds.
+      induction ds as [| [dnm dt] ds' IHds'];
+        intros cl P nm t.
+      - (* ds = nil *)
+        unfold members_ok'. simpl. 
+        exists (is_ok c cl t /\ P).
+        tauto.
+      - (* ds = (dnm, dt) :: ds' *)
+        replace (fst (members_ok' c cl P ((nm, t) :: (dnm, dt) :: ds')))
+        with (fst (members_ok' c (upd_ctxloc cl c nm t) 
+                             (is_ok c cl t /\ P) ((dnm, dt) :: ds')))
+          by (unfold members_ok'; reflexivity).
+        remember (upd_ctxloc cl c nm t) as cl'.      
+        specialize (IHds' cl' (is_ok c cl t /\ P) dnm dt).
+        inversion IHds' as [Ps HPs].
+        inversion HPs as [Heq Himp].
+        exists Ps. split.
+        assumption. tauto.
+    Qed.
+
+    Lemma members_ok'__head_ok :
+      forall (c : ctx) (decls : list (id * dt)) (cl : ctxloc) (initP : Prop)
+             (nm : id) (d : dt),
+        initP ->
+        fst (members_ok' c cl initP ((nm, d) :: decls)) ->
+        (is_ok c cl d) /\ initP.
+    Proof.
+      intros c ds cl P nm t HP H.
+      pose proof (members_ok'__fst_prop c ds cl P nm t) as Hex.
+      inversion Hex as [Ps [Heq Himp]].
+      rewrite Heq in H. apply Himp in H.
+      assumption.
+    Qed. 
+
+    Lemma members_ok'_b__complete :
+      forall (c : ctx) (decls : list (id * dt)) (cl : ctxloc) (initP : Prop),
+        initP ->
+        fst (members_ok' c cl initP decls) ->
+        fst (members_ok'_b c cl decls) = true.
+    Proof.
+      intros c ds.
+      induction ds as [| [nm t] ds' IHds'];
+        intros cl P HP H.
+      - simpl. reflexivity.
+      - (* ds = (nm, t) :: ds' *)
+        assert (H' := H).
+        apply members_ok'__head_ok in H'.
+        inversion H' as [Hok _].
+        assert (Hok' := Hok). apply TOkP.is_ok_b__complete in Hok'.
+        remember (upd_ctxloc cl c nm t) as cl'.
+        replace (members_ok'_b c cl ((nm, t) :: ds'))
+        with (members_ok'_b c cl' ds')
+          by (unfold members_ok'_b; simpl; subst cl'; rewrite Hok'; reflexivity).
+        apply IHds' with (initP := is_ok c cl t /\ P).
+        assumption.
+        unfold members_ok' in *. simpl in *.
+        subst cl'. assumption. assumption.
+    Qed.  
+
+    Lemma members_ok_b__sound :
+      forall (c : ctx) (decls : list (id * dt)),
+      members_ok_b c decls = true ->
+      members_ok c decls.
+    Proof.
+      intros c ds H.
+      unfold members_ok_b in H.
+      unfold members_ok.
+      apply members_ok'_b__sound with (initP := True) in H.
+      assumption. constructor.
+    Qed.
+
+    Lemma members_ok_b__complete :
+      forall (c : ctx) (decls : list (id * dt)),
+        members_ok c decls -> 
+        members_ok_b c decls = true.
+    Proof.
+      intros c ds H.
+      unfold members_ok in H.
+      unfold members_ok_b.
+      apply members_ok'_b__complete with (initP := True) in H.
+      assumption. constructor.
+    Qed.
+
+(* ----------------------------------------------------------------- *) 
+
+    Module MData := MMD.HelperD.MData.
+    Module MDataM <: GenericModule_DataProps 
+                       MId MData MMD.HelperD.MDataM MMI.HelperI.MDataM.
+      Definition members_ok_b__sound := members_ok_b__sound.
+      Definition members_ok_b__complete := members_ok_b__complete.
+    End MDataM.
+    Module M := GenericModule_Props 
+                  MId MMD.HelperD.MData
+                  MMD.HelperD.MDataM MMI.HelperI.MDataM
+                  MDataM.
+
+  End Helper.
+
+(* ================================================================= *)
+(** *** Properties *)
+(* ================================================================= *)
+
+  Theorem module_ok_b__sound : forall (c : ctx) (decls : list (id * dt)),
+      module_ok_b c decls = true ->
+      module_ok c decls.
+  Proof.
+    apply Helper.M.module_ok_b__sound.
+(*    intros c ds. intros H.
+    unfold module_ok_b in H. 
+    unfold module_ok.
+    rewrite -> andb_true_iff in H. inversion H as [Hid Hds].
+    apply MId.IdLS.Props.ids_are_unique__sound in Hid.
+    apply Helper.members_ok_b__sound in Hds.
+    split; assumption. *)
+  Qed.
+
+  Theorem module_ok_b__complete : forall (c : ctx) (decls : list (id * dt)),
+      module_ok c decls ->
+      module_ok_b c decls = true.
+  Proof.
+    apply Helper.M.module_ok_b__complete.
+(*    intros c ds. intros H.
+    unfold module_ok_b.
+    unfold module_ok in H.
+    inversion H as [Hdup Hmems].
+    rewrite -> andb_true_iff. split.
+    apply MId.IdLS.Props.ids_are_unique__complete in Hdup. assumption.
+    apply Helper.members_ok_b__complete. assumption. *)
+  Qed.
+
+End SinglePassModuleProps.
+
+
+
